# 線性轉換
$T:V\rightarrow W$ ($V$, $W$ are vector space)
Null spaces (零空間)
and
Ranges (值域)
## 定義
$T:V\rightarrow W$ ($V$, $W$ are vector space)
T is a linear transformation from $V$ to $W$ (or linear) if
1. $T(x+y)=T(x)+T(y)$ for all $x,y\in V$
2. $T(cx)=cT(x)$ for all $c\in F$, $x\in V$
## Facts:
1. $T(0)=0$
2. $T(x-y)=T(x)-T(y)$
3. $T$ is linear $\Leftrightarrow T(cx+y)=cT(x)+T(y)$ for all $c\in F$, and all $x,y\in V$
### 證明
#### 1
$0+T(0)=T(0+0)=T(0)+T(0)$
$0=T(0)$

---
$T(0)$(向量)$=T(0$(純量)$x)=0T(x)=0$
#### 2
$T(x-y)=T(x+(-1)y)=T(x)+T((-1)y)$   根據def (1)
$=T(x)+(-1)T(y)$  根據def (2)
$=T(x)-T(y)$
#### 3
$(\Rightarrow)$
$T(cx+y)=T(cx)+T(y)$ 根據def (1)
$=cT(x)+T(y)$ 根據def (2)
for all $x,y\in V$ , and $c\in F$
$(\Leftarrow)$
令$c=1$
$T(x+y)=T(x)+T(y)$
令$y=0$
$T(cy+0)=cT(x)+T(0)$
$=cT(x)+0$
$=cT(x)$
### 例子
#### Ex1. $f: V=R^2\rightarrow W=R^3$
$f((a_1,a_2))=(a_1+a_2,1,a_1)$
$f(a_1,a_2)=(a_1+a_2,1,a_1)$ 
---
$T(0,0)=(0,1,0) \Rightarrow$ Not Linear

$f((a_1,a_2))$通常會簡寫成$f(a_1,a_2)$

#### Ex2. $T:R^2 \rightarrow R^2$ , $T(a_1,a_2)=(a_1+a_2,a_1)$
##### pf:
$x=(a_1,a_2)$
$y=(b_1,b_2)$
$T(cx+y)=T(ca_1+b_1,ca_2+b_2)$
$=(ca_1+b_1+ca_2+b_2,ca_1+b_1)$
$=c(a_1+a_2,a_1)+(b_1+b_2,b_1)$
$=cT(x)+T(y)$
#### Ex3. T: $P_n(R)\rightarrow P_{n-1}(R)$ , $T(P(x))=P'(x)$
Claim: 微分是種線性運算

---
Wanted: 
$T(cx+y)=T(cp(x)+q(x))$  
p, q : 多項式
$=c(p(x)+q(x))'$ (' : 微分)

---
$CT(P(x)+T(q(x))$
$=cp'(x)+q'(x)$

---
Wanted:
$(cp(x)+q(x))'=cp'(x)+q'(x)$ (微積分)

#### Ex4.
$T(a_1,a_2)=(2a_1+a_2,3a_2)$
$T(a_1,a_2)=(a_1,0)$
$T(a_1,a_2)=(|a_1|,a_2)$
$T(a_1,a_2)=(Sina_1,a_2)$
$T(a_1,a_2)=(2a_1^2+a_2,3a_2)$
### Facts:
$T: V\xrightarrow{linear}W$
$\left\{\begin{matrix} (a)T(x+y)=T(x)+T(y), \forall x,y\in V\\(b)T(cx)=cT(x), \forall c\in F, x\in V\\\end{matrix}\right.$
或
(c) $T(cx+y)=cT(x)+T(y), \forall c\in F, x,y\in V$

---
i) Ex. 38, 39 \[(a) (b) 2條件互相獨立\]
ii)  $F=Q$ 
$\Rightarrow (a) \Rightarrow (b)$
---
#### pf (ii)
Let $c=\frac{m}{n}$
$n, m\in Z, n\neq 0$
Wanted: $T(\frac{m}{n}x)=\frac{m}{n}T(x)$ 
(a) Claim: $T(mx)=mT(x). m\geq 0, m\in Z$
$T(x+x+...+x)$(m個) $=T(x)+(x+...+x)$(m-1個)

(b) Claim: $T(-x)=-T(x)$
$T(x)=T(2x+(-x))=T(2x)+T(-x)$
$T(x)=2T(x)+T(-x)$
$T(-x)=-T(x)$

(c) $T(mx)=mT(x), m<0, m\in Z$
$T(mx)=T((-m)(-x))$ 
$=(-m)T(-x)$  根據 (a)
$=mT(x)$ 根據 (b)

(d) Claim $T(\frac{x}{n})=\frac{1}{n}T(x)$
$T(\frac{x}{n})=T(x+(-\frac{n-1}{n}x))$
$T(\frac{x}{n})=T(x)+(-n+1)T(\frac{x}{n})$
$\Rightarrow 0=T(x)-nT(\frac{x}{n})$
$nT(\frac{x}{n})=T(x)$
$T(\frac{x}{n})=\frac{T(x)}{n}$

(e) Hence, $T(\frac{m}{n}x)=\frac{m}{n}T(x)$

## Null Space and range
### 定義
>$T:V\xrightarrow{linear}W$
> 1. Null space of $T=N(T)(=ker(T)) = \{x\in V:T(x)=0\}$
> 2. Range of $T = R(T)=\{T(x):x\in V\}=\{y\in W:\exists x$ such that $T(x)=y\}$

### 例子
#### Ex: $T(a_1,a_2)=(2a_1+a_2,3a_2)$ , $V=R^2=W$
##### sol 
$(2a_1+a_2,3a_2)=(0,0)$
$\Rightarrow a_2=0=a_1$
$N(T)=\{(0,0)\}$   子空間
dim($N(T)$) = 0

$R(T)=\{(2a_1+a_2,3a_2): a_1,a_2\in R\}$
$=\{(x,y):x,y\in R\}$
$=R^2$ : 子空間
dim($R(T)$) = 2
#### Ex2: $T(a_1,a_2)=(a_1,0)$, $T:R^2\rightarrow R^2$
這個函數叫projection(投影)
幾何的線性轉換三劍客: projection, reflection, rotation
![[Pasted image 20240831152951.png]]
$N(T)=\{(0,a_2):a_2\in R\}$
= the y-axis 子空間
$\beta=\{(0,1)\}$ dim($N(T)$)=1

---
$R(T)=\{(a_1,0):a_1\in R\}$
$=$ the x-axis
dim($R(T)$) $= 1$
#### Ex.3 $T: R^3\rightarrow R^2$ , $T(a_1,a_2,a_3)=(a_1-a_2,2a_3)$, $N(T)$ ? $R(T)$?
$N(T)=\{(a_1,a_1,0): a_1\in R\}$
dim($N(T)$)=1 ($\beta=\{(1,1,0)\}$)




$R(T)=\{(a_1-a_2,2a_3): a_1,a_2,a_3\in R\}$
$=\{(x,y):x,y\in R\}=R^2$
dim($R(T)$)$=2$



#### Ex.4 $T:P_2(R)\rightarrow M_{2\times2}(R)$ $T(f(x))= \begin{pmatrix} f(1)-f(2) & 0 \\ 0 & f(0) \\ \end{pmatrix}$
for example
$f(x)=x-1$
$T(f(x))=\begin{pmatrix} 0-1 & 0 \\ 0 & -1 \\ \end{pmatrix} = \begin{pmatrix} -1 & 0 \\ 0 & -1 \\ \end{pmatrix}$
$f(x)=x^2+x+1$
$T(f(x))=\begin{pmatrix} 3-7 & 0 \\ 0 & 1 \\ \end{pmatrix}=\begin{pmatrix} -4 & 0 \\ 0 & 1 \\ \end{pmatrix}$
prove $T(cf(x)+g(x)) = cT(f(x))+T(g(x))$
$T(f(x))=\begin{pmatrix} 0 & 0 \\ 0 & 0 \\ \end{pmatrix}$
$=\begin{pmatrix} f(1)-f(2) & 0 \\ 0 & f(0) \\ \end{pmatrix}$
$\Rightarrow \left\{\begin{matrix} f(1)-f(2)=0 \\ f(0)=0 \end{matrix}\right.$ 
$f(x)=ax^2+bx+c$
$c=0$
$a+b+c=4a+2b+c$
$\Rightarrow b=-3a$
$N(T)=\{ax^2-3a\ ,\ x:\ a\in R\}$
$N(T)$: a subspace of $P_2(R)$
$\beta=\{x^2-3x\}$
dim($N(T)$)=1
$R(T)=\{\begin{pmatrix} f(1)-f(2) & 0\\ 0 & f(0)\\\end{pmatrix}\ :f\in P_2(R)\}$
$=\{\begin{pmatrix}a_1 & 0 \\ 0 & a_2\\\end{pmatrix}\ : a_1,a_2\in R$
$=$ The set of diagonal matrix of size $2\times2$ (對角線矩陣)
$\beta=\{\begin{pmatrix}1 & 0 \\ 0 & 0\\\end{pmatrix},\begin{pmatrix}0 & 0 \\ 0 & 1\\\end{pmatrix}\}$
dim($R(T)$)=2
## Thm 2.1
$T:V\xrightarrow{linear}W$
$\Rightarrow \begin{matrix} N(T) \\ R(T)\\\end{matrix}$ is a subspace of $\begin{matrix}V\\W\\\end{matrix}$
### pf: 是否子空間只需檢查封閉性
($T(0)=0$ $\Rightarrow N(T)$ and $R(T)$ are nonempty!
1. $x+y\in N(T)$ whenever $x,y \in N(T)$
2. $cx\in N(T)$ whenever $x\in N(T)$ and $c\in F$
$x,y\in N(T)$
$\Rightarrow T(x)=T(y)=0$
$0=T(x)+T(y)=T(x+y)$
$\Rightarrow x+y\in N(T)$
$x\in N(T)$
$\Rightarrow T(x)=0$
$cT(x)=c0=0$
$T(cx)=0$
$\Rightarrow cx\in N(T)$
值域正法雷同
## Thm 2.2
>Let $\beta =\{v_1,...,v_n\}$ be a basis of $V$. 
>Then $R(T)=$Span($T(\beta)$)$=$Span$\{T(v_1),T(v_2),...T(v_n)\}$

![[Pasted image 20240831165427.png]]
### 證明
 $R(T)=$Span($T(\beta)$)$=$Span$\{T(v_1),T(v_2),...T(v_n)\} = K$
Wanted: $R(T)=K$
1. $R(T)\supset K$
$\{T(v_1),...,T(v_n)\}\subset R(T)$
$\Rightarrow K\subset R(T)$ (Thm 2.1)

2. $R(T)\subset K$
Wanted:  If $y\in R(T)$, then $y\in K$
**pf:** if $y\in R(T), \Rightarrow \exists x \in V$, such that  $T(x)=y$
$\Rightarrow x=\sum^{n}_{i=1}c_iv_i$, for some $c_i\in F$
$\Rightarrow T(x)=T(\sum^{n}_{i=1}c_iv_i)=\sum^{n}_{i=1}c_iT(V_i)$ (定義)
$\Rightarrow y=T(x)\leftarrow$Span$\{T(v_1),...,T(v_n)\}=K$
## Thm 2.3
$T:V\xrightarrow{linear}W$, dim($V$)$<\infty$ , 
$\Rightarrow$ dim($N(T)$) $+$ dim($R(T)$)$=$ dim($V$)
( def ) ( Nullity($T$) $+$ Rank($T$) $=$ dim($V$) )
### 證明
Let dim($N(T)=P$ dim($V$)$=n(n\geq p)$ and $\beta=\{v_1,...,v_p\}$ be a basis for $N(T)$.
and $\gamma=\{v_1,...,v_p,v_{p+1},...,v_n\}$ be a basis for $V$
![[Pasted image 20240831222846.png]]
Wanted: dim($R(T)$)$=n-p$
$X=\{T(v_{p+1}),T(v_{p+2}),...,T(v_n)\}$ is a basis for $R(T)$ 
Wanted:
1. Span($X$) = $R(T)$
2. $X$ is linear independent

**根據 Thm2.2**
$R(T)=$Span$\{T(v_1),T(v_2),...,T(v_p),T(v_{p+1}),...,T(v_n)\}$


$=$Span$\{0,0,...,0,T(v_{p+1}),...,T(V_n)\}$
$=$Span$\{T(v_{p+1}),...,T(V_n)\}$ (1. 達成)
2. Suppose $\sum_{i=1}^{n-p}c_{p+i}T(v_{p+i})=0$
($c_{p+1}T(v_{p+1})+c_{p+2}T(v_{p+2})+...+c_nT(v_n)=0$)
Claim: $c_{p+1}=c_{p+2}=...=c_n=0$
**T:linear** $\Rightarrow T(\sum_{i=1}^{n-p}c_{p+i}v_{p+i})=0$
$\Rightarrow \sum c_{p+i}v_{p+i} \in N(T)$
$\Rightarrow \sum_{i=1}^{n-p}c_{p+i}v_{p+i}=c_1v_1+c_2v_2+...+c_pv_p$
$\Rightarrow c_1v_1+...+c_pv_p+c_{p+1}v_{p+1}+...+c_nv_n=0$
$c_1=c_2=...=c_n=0$

## Thm 2.4
$T: V\xrightarrow{linear} W$
$T$ is 1-1$\Leftrightarrow N(T)=\{0\}$ 
Remark: The Thm is true for $V$ and $W$ being infinite-Dimensional.

### Pf
$(\Rightarrow)$
已知$T$: 1-1 & linear
求證: $N(T)=\{0\}$
 ![[Pasted image 20240902150835.png]]
Since $T(0)=0$ and $T$ is 1-1, $N(T)=\{0\}$
$(\Leftarrow)$
If $T(x)=T(y)\Rightarrow x=y$
Let $T(x)=T(y) \Rightarrow T(x)-T(y)=0$
$T$ is linear $\Rightarrow$ $T(x-y)=0 \Rightarrow x-y \in N(T)=\{0\}$  
$\Rightarrow x-y=0 \Rightarrow x=y \Rightarrow T$ is 1-1

## Thm 2.5
>*  $T: V\xrightarrow{linear}W$
>* dim($V$)$=$ dim($w$)$<\infty$
>TFAE(The following are equivalant)
>1. T is 1-1
>2. T is onto ($R(T)=W$)
>3. dim($V$)$=$ rank($T$)

 Remarks: 
1. $T$ is nonlinear $\Rightarrow$ the contention of the theorem fail.
2. If $V, W$are not finite dimensional$\Rightarrow$ the contention of the theorem fail.
### Pf
1.$\Rightarrow$ 2.
因為 $T$ is 1-1 $\Rightarrow$(Thm2.4) $N(T)=\{0\}$
$\Rightarrow$ dim($N(T)$)$=$Nullity of $T=0$
$\Rightarrow$(Thm2.3)dim($R(T)$) $=$ rank($T$)$=$dim($V$)=dim($W$)
Since $R(T)$ is a subspace of $W$,
$R(T)=W$
2.$\Rightarrow$ 3.
因為 $R(T)=W$, dim($W$)=dim($V$)
$\Rightarrow$ dim($R(T)$)=dim($V$)
(Thm2.3)$\Rightarrow$ Nullity($T$)=0
(Thm2.3)$\Rightarrow$dim($V$)=rank($T$)
3.$\Rightarrow$ 1.
(Thm2.3) $\Rightarrow$ Nullity($T$)$=0$
$\Rightarrow N(T)=\{0\}$
(Thm2.4)$\Rightarrow T$ is 1-1 
## Thm2.6
>Let $\beta = \{u_1,...,u_n\}$ be a basis for $V$ and $W_i\in W$ , $i=1,2,...,n$ . Then $\exists$ linear transformation $T$ such that
>1. $T$ is linear
>2. $T(u_i)=w_i$
>3. $T$ is  unique
(掌握基底的行為，掌握全世界)
### Pf
Let $v\in V \Rightarrow \exists!$ scalar $a_i$ such that $v=a_1u_1 + a_2u_2 + ... + a_nu_n$  
Define $T$ such that $T(v)=a_1w_1+...+a_nw_n$
Claim: 
1. $T$ is linear 
2. $T(u_i)=w_i$
3. $T$ is unique
---
$v=u_i$
$=0u_1+...+0u_{i-1}+1u_i+0u_{i+1}+...+0u_n$

# Matrix Representation of a Linear Transformation
## 定義
> 1. An ordered basis for $V$ , where dim($V$) $<\infty$
>    $\beta = \{u_1,u_2,...,u_n\}\neq \beta'=\{u_2,u_1,u_3,...,u_n\}$
> 2.  Let $\beta=\{u_1,u_2,...,u_n\}$ be an ordered basis for  $V$, let $x\in V$ and $x=a_1u_1+a_2u_2+...+a_nu_n$. Then $\begin{bmatrix}a_1 \\ a_2\\...\\ a_n\end{bmatrix}$ is called the coordinate vector of $x$ with relative to $\beta$
> 3. $T:V\xrightarrow{linear} W$, let $\beta=\{u_1,...,u_n\}$ and $\gamma=\{v_1,...,v_m\}$ be ordered basis for $V$ and $W$ , respectingly. Let $T(u_j)=\sum_{i=1}^{m}a_{ij}v_i$, $j=1,...,n$. e.g. $T(u_1)=a_{11}v_1+a_{21}v_2+...+a_{m1}v_m$
>    Let $A=(a_{ij})$, $1\leq i\leq m,1\leq \gamma\leq n$
>    Then $A$ of dimension $m\times n$, is called the matrix represation of $T$ with respect to $\beta$ and $\gamma$.
>    We shall denote by $A=\begin{bmatrix}T\\\end{bmatrix}^\gamma_\beta$. If $V=W$ and $\beta=\gamma$, then we shall denote by $A=\begin{bmatrix}T\\\end{bmatrix}_\beta$



## 例子
$V=p_2(R)$
$\beta=\{1,x,x^2\}$
$v\in V$
![[Pasted image 20240902172527.png]]
$-2+3x+x^2$: vector coordinate with respect to $\beta\Rightarrow\begin{bmatrix}v\\\end{bmatrix}_\beta = \begin{pmatrix}-2\\3\\1\\\end{pmatrix}$ 
$\beta'=\{1,x^2,x\} \Rightarrow \begin{bmatrix}v\\\end{bmatrix}_{\beta'}\begin{pmatrix}-2\\1\\3\\\end{pmatrix}$
We shall denote $\begin{bmatrix}a_1\\a_2\\...\\a_n\\\end{bmatrix}$ by $\begin{bmatrix}x\\\end{bmatrix}_\beta$
## 例子
### Ex1.
$T:R^2\rightarrow R^3$
$T(a_1,a_2)=(a_1+a_2,a_2-a_1,a_1+3a_2)$
$\beta=\{(1,0),(0,1)\}$
$\gamma=\{(1,0,0),(0,1,0),(0,0,1)\}$
$\begin{bmatrix}T\\\end{bmatrix}^\gamma_\beta$ $=\begin{pmatrix}1 & 1\\ -1&1\\1&3\\\end{pmatrix}_{3\times2}$
$T(1,0)=(1,-1,1)=1(1,0,0)-1(0,1,0)+1(0,0,1)$
$T(0,1)=(1,1,3)=1(1,0,0)+1(0,1,0)+3(0,0,1)$
### Ex.2
$T:P_2(R)\rightarrow R$ and $T(f(x)=f(2)$ \[$P_2(R)$\=$V$，$R$=$W$]
$\beta=\{1,x,x^2\}$
$\gamma=\{1\}$
e.g: $f(x)=x^2$ ，$T(x^2)=4$
$\begin{bmatrix}T\\\end{bmatrix}= \begin{bmatrix}1&2&4\\\end{bmatrix}_{1\times3}$

### Ex.3
$T:P_2(R)\rightarrow M_{2\times2}(F)$
by 
$T(f(x))=\begin{pmatrix}f'(0) & 2f(1)\\0 & f''(3)\\\end{pmatrix}$
$\beta=\{1,x,x^2\}$
$\gamma=\{\begin{pmatrix}1&0\\0&0\\\end{pmatrix},\begin{pmatrix}0&1\\0&0\\\end{pmatrix}\begin{pmatrix}0&0\\1&0\\\end{pmatrix}\begin{pmatrix}0&0\\0&1\\\end{pmatrix}\}$
$T(1) = \begin{pmatrix}0&2\\0&0\\\end{pmatrix}= 0\begin{pmatrix}1&0\\0&0\\\end{pmatrix}+2\begin{pmatrix}0&1\\0&0\\\end{pmatrix}+0\begin{pmatrix}0&0\\1&0\\\end{pmatrix}+0\begin{pmatrix}0&0\\0&1\\\end{pmatrix}\}$
$T(x) = \begin{pmatrix}1&2\\0&0\\\end{pmatrix}= 1\begin{pmatrix}1&0\\0&0\\\end{pmatrix}+2\begin{pmatrix}0&1\\0&0\\\end{pmatrix}+0\begin{pmatrix}0&0\\1&0\\\end{pmatrix}+0\begin{pmatrix}0&0\\0&1\\\end{pmatrix}\}$
$T(x^2) = \begin{pmatrix}0&2\\0&2\\\end{pmatrix}= 0\begin{pmatrix}1&0\\0&0\\\end{pmatrix}+2\begin{pmatrix}0&1\\0&0\\\end{pmatrix}+0\begin{pmatrix}0&0\\1&0\\\end{pmatrix}+2\begin{pmatrix}0&0\\0&1\\\end{pmatrix}\}$
$\Rightarrow\begin{bmatrix}T\\\end{bmatrix}^\gamma_\beta=\begin{pmatrix}0&2&0&0\\1&2&0&0\\0&2&0&2\\\end{pmatrix}_{4\times3}$

## 定義
>1. $\mathfrak{L}(V,W)=\{T: T:V\xrightarrow{linear} W$，$V$ and $W$ are vector spaces$\}$
>2. If $V=W$，then we write $\mathfrak{L}(V,V)$ as $\mathfrak{L}(V)$

## Thm2.7
>$\mathfrak{L}(V,W)$ is a vector space.
>(Defs: $U,T\in \mathfrak{L}(v,w)$
>$(U+T)(x)=U(x)+T(x)$ ， $x\in V$
>$F$和$V$及$W$的$F$是一樣
>Let $\alpha\in F$，$T\in\mathfrak{L}(V,W)$
>$(\alpha T)(x)=\alpha T(x)$
### 證明
(加法封閉性)
$(U+T):V\rightarrow w$ (of course!)
欲證:$U+T$仍為線性 For any $\alpha\in F$，$\forall x,y\in V$
[$Q=U+T$]
$Q((\alpha x+y)=$(wanted)$\alpha Q(x)+Q(y)$
$=U(\alpha x+y)+T(\alpha x+y)=\alpha U(x)+U(y)+\alpha T(x)+T(y)$
$=\alpha[U(x)+T(x)]+[U(y)+T(y)]$
(乘法封閉性)
Wanted: $\alpha T$: linear
$(\alpha T)(x)=\alpha T(x)$
$\Leftrightarrow(\alpha T)(cx+y)=c(\alpha T)(x)+(\alpha T)(y)$
for all $c\in F$，$x,y\in V$
(V 1)
$U+T=T+U$
 $\Rightarrow (U+T)(x)=(T+U)(x)$ for all $x\in V$
$U(x)+T(x)=T(x)+U(x)$ 
因為$T(x)$和$U(x)$都屬於$W$，所以有交換律的性質
## Thm 2.8
>$T,U: V\xrightarrow{linear}W$
>1. $[T+B]_\beta^\gamma=[T]^\gamma_\beta+[U]^\gamma_\beta$ 
>2. $[\alpha T]^\gamma_\beta=\alpha[T]_\beta^\gamma$
### 證明
定義

### 例子
$R^2\rightarrow R^3$
$T(a_1,a_2)=(a_1+3a_2,0,2a_1-4a_2)$
$U(a_1,a_2)=(a_1-a_2,2a_1,3a_1+2a_2)$
$R^2\rightarrow \beta=\{(1,0),(0,1)\}$
$R^3\rightarrow\gamma=\{(1,0,0),(0,1,0),(0,0,1)\}$
$(T+U)(a_1,a_2)=(2a_1+2a_2,2a_1,5a_1-2a_2)$
$[T]^\gamma _\beta=\begin{bmatrix}1&3\\0&0\\2&-4\\\end{bmatrix}$ ，$[U]^\gamma_\beta=\begin{bmatrix}1&-1\\2&0\\3&2\\\end{bmatrix}$
$[T]^\gamma_\beta+[U]=\begin{bmatrix}2&2\\2&0\\5&-2\\\end{bmatrix}$

# 合成函數
![[Pasted image 20240903171739.png]]
$U\circ T=UT$
$(UT)(x)=U(T(x))$
(註: 大部分函數沒有定義函數相乘)
## Thm2.9
$UT:$ linear provided
$U$ and $T$ are linear
### 證明
Needed: $(UT)(\alpha x+y)=\alpha(UT)(x)+(UT)(y)$
for all $x,y\in V$，$\alpha \in F$
$(UT)(\alpha x+y)=U(T(\alpha x+y))$
$(UT)(\alpha x+y)=U(T(\alpha x+y))$
($T$ is linear)$=U(\alpha T(x)+T(y))$
($U$ is linear)$=\alpha U(T(x))+U(T(y))$
$=\alpha (UT)(x)+(UT)(y)$

## Thm2.10
>$U,T,U_i,T_i$: linear
以下符號有意義
>1. $(T_1+T_2)U=T_1U+T_2U$
>2. $T(U_1+U_2)=TU_1+TU_2$
>3. $(TU_1)U_2=T(U_1U_2)$
>4. $TI=IT=T$
(問: 那些結論需要線性函數)
### 證明
#### 1. $(T_1+T_2)U=T_1U+T_2U$
Needed: $((T_1+T_2)U)(x)=(T_1U+T_2U)(x)$ for all $x\in V$ 
$((T_1+T_2)U)(x)$
$=((T_1+T_2))(U(x))=(T_1+T_2)(U(x))$
$=T_1(U(x))+T_2(U(x))$
$=(T_1U)(x)+(T_2U)(x)$
$(T_1U+T_2U)(x)$
## 定義
>$A=(A_{ij})_{m\times n}$ $B=(B_{ij})_{n\times p}$
  Define $AB=C=(c_{ij})_{m\times p}$ as $c_{ij}=A$的第i列和B第j行的內積
>$=\sum^{n}_{k=1}A_{ik}B_{kj}$
### 例子
$A=\begin{pmatrix}1&1&1\\2&2&2\\\end{pmatrix}_{2\times3}$
$B=\begin{pmatrix}1&1&1\\2&2&2\\3&3&3\\\end{pmatrix}_{3\times3}$
...

## 矩陣相乘性質
>1. $(AB)^t=B^tA^t$
>2. Thm2.12
>(a.) $A(B_1+B_2)=AB_!+AB_2$
>(b.)$(A_1+A_2)B=A_1B+A_2B$
>(c.) $a(AB)=A(aB)=(aA)B$ for all $a\in F$
>(d.) $I_mA_{m\times n}=A_{m\times n}I_n=A$
>$I_n=\begin{pmatrix}1&...&0&0\\0&1&...&0\\0&...&...&1\\\end{pmatrix}_{n\times n}$
>(方陣, n=m)
>Thm2.13
>3. $AB=A(b_1,...,,b_p)$ (Block Multiple)
>$=(Ab_1,...,Ab_p)$
>Here  $A: m\times n$ $B: n\times p$
>and $B=(b_1,b_2,...,b_p)$
>4. $AB\neq BA$ (AB通常不等於BA)
>5. $AB=0$(零矩陣) 不見得 $A=0$或$B=0$
### 證明
$A=(A_{ij})_{m\times n}$
transpose: $A^t=(A_{ji})_{n\times m}$  (行列位置對調)
e.g. $A=\begin{pmatrix}1&1&1\\2&2&3\\\end{pmatrix}$ $A^T=\begin{pmatrix}1&2\\1&2\\1&3\end{pmatrix}$
$B^t=(B_{ji}){p\times n}$
Let $AB=C=(C_{ij})_{m\times p}$
$(AB)^t=(C_{ji})$
$C_{ij}=(def)\sum^{n}_{k=1}A_{ik}B_{kj}$
$C_{ji}=\sum^{n}_{k=1}A_{jk}B_{ki}$
$=\sum^{n}_{k=1}B_{ki}A_{jk}$
$=\sum^n_{k=1}(B^t)_{ik}(A^t)_{kj}$
$\Rightarrow(AB)^t=B^tA^t$
## Thm 2.11
![[Pasted image 20240903225343.png]]
$\Rightarrow [UT]^\gamma_\alpha=[U]^\gamma_\beta[T]^\beta_\alpha$
線性的合成函數的矩陣=個別線性函數的矩陣相乘
### 例子
$T(a_1,a_2)=(a_1+a_2,a_1-a_2)$
$U(a_1,a_2)=(a_2,a_1)$
$\alpha=\beta=\gamma=\{(1,0),(0,1)\}$
$C=UT(a_1,a_2)=U(T(a_1,a_2))=U(a_1+a_2,a_1-a_2)$
$=(a_1-a_2,a_1+a_2)$
$C(a_1,a_2)=(a_1-a_2,a_1+a_2)$
$[C]_\alpha=\begin{bmatrix}1&-1\\1&1\\\end{bmatrix}$
$C(1,0)=(1,1)=1(1,0)+1(0,1)$
$C(0,1)=(-1,1)=-1(1,0)+1(0,1)$
$\begin{bmatrix}0&1\\1&0\\\end{bmatrix}\begin{bmatrix}1&1\\1&-1\\\end{bmatrix}=\begin{bmatrix}1&-1\\1&1\\\end{bmatrix}$

$C(u_j)=UT(u_j)=U(T(u_j))$
(def)$=U(\sum^m_{k=1}B_{kj}v_k)=$(線性)$\sum^m_{k=1}B_{kj}U(v_k)$
(def)$=\sum^m_{k=1}B_{kj}(\sum^p_{i=1} A_{ik}S_i)$
$=\sum^m_{k=1}\sum^p_{i=1}B_{ij}A_{ik}S_i$
(交換)$=\sum^p_{i=1}\sum^m_{k=1}B_{kj}A_{ik}S_i$
$=\sum^p_{i=1}(\sum^m_{k=1}A_{ik}B_{kj})S_i$
$=\sum^p_{i=1}c_{ij}S_i$
## Thm 2.14
>$T:V\xrightarrow{linear} W$(ordered basis: V:$\beta$、W:$\gamma$)，dim($V$)$<\infty$
>dim($W$)$<\infty$ $\Rightarrow[T(v)]_\gamma=[T]^\gamma_\beta[v]_\beta$，$v\in V$ ($[T(v)]_\gamma$，$T(v)$的向量表示法)
### 例子 
#### Ex: $T:P_3(R)\rightarrow P_2(R)$ (V,W)
$T(f(x))=f'(x)$
$\beta=\{1,x,x^2,x^3\}$
$\gamma=\{1,x,x^2\}$
let $v=x^3-2x^2+x-1$
$T(v)=3x^2-4x+1=1*1+(-4)x+(3)x^2$
$[T(v)]_\gamma=\begin{bmatrix}1\\-4\\3\\\end{bmatrix}$，$[T]^\gamma_\beta=(A_{ij})_{3\times4}$
$[v]_\beta=\begin{bmatrix}-1\\1\\-2\\1\\\end{bmatrix}$
$T(1)=0=0*1+0*x+0*x^2$
$T(x)=1=1*1+0*x+0*x^2$
$T(x^2)=2x=0*1+2*x+0*x^2$
$T(x^3)=1=0*1+0*x+3*x^2$

$A=\begin{pmatrix}0&1&0&0\\0&0&2&0\\0&0&0&3\end{pmatrix}$
$\begin{pmatrix}1\\-4\\3\\\end{pmatrix}=\begin{pmatrix}0&1&0&0\\0&0&2&0\\0&0&0&3\\\end{pmatrix}\begin{pmatrix}-1\\1\\-2\\1\\\end{pmatrix}$
### 證明
#### 方法一(按照定義)
...
#### 方法二(Tricky)
For fix $v\in V$，define $f:F\rightarrow V$ and $g: F\rightarrow W$ by $f(a)=av$，$g(a)=aT(v)$，where $a\in F$
$V: \beta=\{v_1,...,v_n\}$
$W: \gamma=\{u_1,...,u_m\}$
![[Pasted image 20240904111134.png]]
$g=Tf$
$Tf(a)=T(f(a))$
$=T(av)=aT(v)$
$=g(a)$
$[T(v)]_\gamma=[g(1)]_\gamma=[g]^\gamma_\alpha$   ， ($[g(1)]_\gamma\rightarrow m$維度的向量，$[g]^\gamma_\alpha\rightarrow m\times 1$的矩陣)
$=[T]^\gamma_\beta[f]^\beta_\alpha$
$=[T]^\gamma_\beta[f(1)]_\beta=[T]^\gamma_\beta[v]_\beta$
## Thm 2.15
> $A:m\times n$矩陣
> $L_A: F^n\rightarrow F^m$  $L_A(x)=Ax$ (a left-multiplication transformation)
> $\beta: \gamma$ standard ordered basis for $F^n$ nad $F^m$
> $\beta=\{\begin{pmatrix}1\\0\\0\\...\\0\\\end{pmatrix}n個\begin{pmatrix}0\\0\\0\\...\\1\\\end{pmatrix}\}$
> $\gamma=\{\begin{pmatrix}1\\0\\0\\...\\0\\\end{pmatrix}m個\begin{pmatrix}0\\0\\0\\...\\1\\\end{pmatrix}\}$
> $\Rightarrow$(a) $[L_A]^\gamma_\beta=A$
> (b) $L_A=L_B\Rightarrow A=B$
> (c) $L_{A+B}=L_A+L_B$ and $L_{aA}=aL_A$ for all $a\in F$
> (d) $T:F^n\rightarrow F^m$ is linear $\Rightarrow\exists!C m\times n$矩陣，such that $T=L_c$. In fact $C=[T]^\gamma_\beta$ 
> (e) $L_{AE}=L_AL_E$
> (f) $m=n$，$\Rightarrow L_{I_n}=I_{F^n}$
 
### 證明
#### a. : Wanted: $[L_A]^\gamma_\beta=A$
 Let: $\beta=\{e_1,...e_n\}$
 $\gamma=\{\bar e_1,...,\bar e_m\}$
$L_A(e_j)=Ae_j=\begin{pmatrix}A_{1j}\\A_{2j}\\...\\A_{mj}\\\end{pmatrix}=A_{1j}\bar e_1+...+A_{mj}\bar e_m$
$\Rightarrow[L_A]^\gamma_\beta=A$
#### d.
$[T(x)]_\gamma=[T]^\gamma_\beta[x]_\beta$
$V=F^n$，$W=F^m$
$[x]_\beta=x$
$x\in F^3\Rightarrow x=\begin{bmatrix}x_1\\x_2\\x_3\\\end{bmatrix}= x_1\begin{bmatrix}1\\0\\0\\\end{bmatrix}+x_2\begin{bmatrix}0\\1\\0\\\end{bmatrix}+x_3\begin{bmatrix}0\\0\\1\\\end{bmatrix}$
$\beta=\{\begin{pmatrix}1\\0\\0\\\end{pmatrix},\begin{pmatrix}0\\1\\0\\\end{pmatrix},\begin{pmatrix}0\\0\\1\\\end{pmatrix}\}$
因為$\beta$,$\gamma$, standard ordered basis
$\Rightarrow[x]_\beta=x$ and $[T(x)]_\gamma=T(x)$
$\Rightarrow T(x)=[T]^\gamma_\beta x$
另$C=[T]^\gamma_\beta$
The uniquences follows from (b)

#### e.
Wanted: $L_{AE}=L_AL_E$ ($A: m\times n$、$E: n\times p$) (兩函數的合成)
$L_{AE}(x)=(L_AL_E)(x)$ for $\forall x\in F^p$
$L_{AE}(x)=AE(x)=A(Ex)$
$=L_A(E_x)=L_A(L_E(x))=(L_AL_E)(x)$
for any $x\in F^p$
## 應用
### 名詞
Graph: 頂點，directed edges(有方向的邊)
![[Pasted image 20240904143816.png]]
Complete Graph : 任兩點都有互通
### 問題: Clique
**Clique:** a (maximum) complete subgraph in a graph
### Hard Problems
1. Finding a clique(數量大時)
2. Listing all clique(數量大時)
Incidence matrix
$\begin{bmatrix}0&1&1&1\\1&0&1&1\\1&1&0&1\\0&1&1&0\\\end{bmatrix}_{4\times4}$
可回答問題:
1. 從1到3兩佈内可以走到的方法
$A^2=AA$
$=\sum_{k=1}^4A_{1k}A_{k3}$
$A_{11}A_{13}+...+A_{14}A_{43}$
$(A+A^2+...+A^m)_{ij}$
= 從i到j m步內可到的走法

問: 給i，$i\in$ a clique?
$A\rightarrow B=\{\begin{matrix}1& if\ A_{ij}=A_{ji}=1\\0& otherwise\\\end{matrix}.$
$B=\begin{pmatrix}0&1&1&0\\1&0&1&1\\1&1&0&1\\0&1&1&0\\\end{pmatrix}$
$i\in$ a clique$\Leftrightarrow (B^3)_{ii}>0$  (Ex.19(or 21))(Tips: 用矩陣乘法)
### 問題: Dominate Graph
$\forall i，j$
$a_{ij}=1\Leftrightarrow A_{ji}=0$
$A_{13}=1$，$A_{31}=0$
$A=\begin{pmatrix}0&1&0&1&0\\0&0&1&0&0\\1&0&0&1&0\\0&1&0&0&1\\1&1&1&0&0\\\end{pmatrix}$
#### Facts: (Tip:用圖的方式去解)
(Ex21)
1. $\exists i$ such that $i$在2步內能reach到其他點
2. $\exists j$，j在2步內被其他點找到

1. $\exists i$(列) such that. $A+A^2$ 的第$i$列的元素$>0$(除了對角線)
2. $\exists j$(行) such that. $A+A^2$ 的第$j$行的元素$>0$(除了對角線)

# Inventibility & Isomophisms
若$V,W$: 向量空間，且dim($V$)=dim($W$)$<\infty$，
則$V$and $W$ "可看成"是一樣
"可看成一樣": 數學上指 $\exists T:V\xrightarrow{linear\ inventible}W$
 $T:V\xrightarrow{linear inventible}W$ (可逆)
V~W Isomophic
## 定義
![[Pasted image 20240904155328.png]]
>$T:V\xrightarrow{}W$ is inventible. $\exists U:W\rightarrow V$ such that 
>(* -1) $UT=I_V$ ($I_V$: $v\rightarrow v$；$I_V(u)=v$)
 and 
  (* -2) $TU=I_W$ ($I_W:\ W\rightarrow W,\ I_W(w)=w$)

Remarks:
1. $U$ is unique! Hence, we may write $U$ as $T^{-1}$
Why?
Let $U_1$, $U_2$ satify(*-1) and (*-2)
Wanted: $U_!=U_2\Leftrightarrow U_1(w)=U_2(w)$，for all $w\in W$
$U_1(w)=U_2T(U_1(w))=U_2((TU_1)(w))=U_2(I_w(w))=U_2(w)$
2. $T:$ $V\rightarrow W$ inventible$\Leftrightarrow$ $T$ is 1-1and onto!
3. $T_1,T_2$: inventible and $T_1,T_2$ is well-defined, Then$(T_1T_2)^{-1}=T_2^{-1}T_1^{-1}$
Step1. T1 T2: inventible
Step2. $(T_1T_2)^{-1}=T_2^{-1}T_1^{-1}$
4. $T:V\xrightarrow{linear\ inventible}W$，$\Leftrightarrow$ so are $T^{-1}$
(Thm2.17)
pf. of  Thm 2.17
![[Pasted image 20240904161530.png]]
(a) Claim: $T^{-1}: W\rightarrow V$ is linear
Let $w_1,w_2\in W$ and $a\in F$
Wanted: $T^-1(aw_1+w_2)=aT^{-1}(w_1)+T^{-1}(w_2)$
$\Rightarrow \exists v_1$ and $v_2\in V$ such that $T(v_1)=w_1$，$T(v_2)=w_2$
$T^{-1}(aw_1+w_2)=T^{-1}=T^{-1}(aT(v_1)+T(v_2))$
$=T^{-1}(T(av_1+v_2))=av_1+v_2$
$=aT^{-1}(w_1)+T^{-1}(w_2)$
$T^{-1}:$ inventible of course! 
## 定義
> A: an $n\times n$ matrix
> A is inventible if $\exists B:n\times n$ matrix such that $AB=BA=I$

Remark: Such B is unique! 
Hence we may write $B$ as $A^{-1}$
$F^4:$ dim 
$M_{2\times 2}(F)$
$P_3(F)$
#### Lemma: 
$T:\ V\xrightarrow{linear\ inventible} W$
Then dim($v$)$<\infty\Leftrightarrow$ dim($w$)$<\infty$
#### Pf. 
$(\Rightarrow)$ Since dim($v$)$<\infty$ ，let $\beta=\{v_1,...,v_n\}$ be a ordered basis for $V$
$\Rightarrow$ $R(T)=$span$\{T(v_1),...T(v_n)\}$
因為T is inventible 
$\Rightarrow W=$span $\{T(v_1),...,T(v_n)\}$
$\Rightarrow$dim($w$)$<\infty$
$(\Leftarrow)$將$T$ is $T^{-1}$ ，做同樣的分析

## Thm 2.18
$T:v\xrightarrow{linear\ inventible}w$($v:\beta,w:\gamma$)，dim($v$), dim($w$)是有限。Then $T$ is inventible$\Leftrightarrow[T]^\gamma_\beta$ is inventible. In this case
$[T^{-1}]^\beta_\gamma=([T]^\gamma_\beta)^{-1}$
### 證明
$(\Rightarrow)$
$T:$ inventible$\Leftrightarrow T$ is 1-1 and onto
Dim($v$)=(Dimensio Thm. 1-1) Rank($T$) $=$(onto)=dim($W$)
Wanted: $[T]^\gamma_\beta$  is inventible
$\Rightarrow \exists:U:W\rightarrow V$ such that
$UT=I_V\Rightarrow [UT]_\beta=[U]^\beta_\gamma[T]^\gamma_\beta$
$=[I_V]_\beta=I_n$
and
$TU=I_W$
同理 $[T]^\gamma_\beta[U]^\beta_\gamma=[I_w]_\gamma=I_n$
$\Rightarrow[T]^\gamma_\beta$ has an inverse $[U]^\beta_\gamma=[T^{-1}]^\beta_\gamma$
$\Rightarrow([T]^\gamma_\beta)^{-1}=[T^{-1}]^\beta_\gamma$
$(\Leftarrow)$
Let $[T]^\gamma_\beta=A$，and $A^{-1}=B$
Let $\beta=\{v_1,...v_n\}$ and $\gamma=\{w_1,...,w_n\}$
問題: 如何找U由B? U的行為可由基底的行為來決定。
$\exists!U:W\xrightarrow{linear}V$ such that $U(w_j)=\sum^n_{i=1} B_{ij}v_i$ (Thm2.6)
($[U]^\beta_\gamma=B$) such that $[UT]_\beta=[U]^\beta_\gamma[T]^\gamma_\beta=BA=I_n=[I_v]_\beta$
$\Rightarrow UT=I_V$ 同理$TU=I_W$
## 定義
>$V$ is isomorphic to $W$, $V$~$W$, if $\exists T:V\xrightarrow{linear\ inventible}W$ 
  such $T$ is called an isomorphism from $V$ to $W$. (If $V$~$W$, then $W$~$V$)

### 例子
$V=P_(F)$
$W=M_{2\times2}(F)$
$V$~$W$
or $f\in P_3,\ T(f)=\begin{pmatrix}f(1)&f(2)\\f(3)&f(4)\\\end{pmatrix}$
$T$ is linear & 
$T(a+bx+cx^2+dx^3)=\begin{pmatrix}a&b\\c&d\\\end{pmatrix}= \begin{pmatrix}0&0\\0&0\\\end{pmatrix}$ inventible!
$\Rightarrow N(T)=\{$ 0多項式$\}$
## Thm2.19 
dim($V$)，dim($W$)$<\infty$
Then $v$~$w\Leftrightarrow$ dim($V$)=dim($W$)
### Pf
$(\Rightarrow)$
$\exists T:V\xrightarrow{linear\ inventible}W$
dim($V$)=Rank($T$)=(onto)dim($W$)
$(\Leftarrow)$
Let $\beta=\{v_1,...,v_n\}$，$\gamma=\{w_1,...,w_n\}$ basis for $v$, $w$ 。
$\Rightarrow \exists!T: v\xrightarrow{linear}w$
such that $T(v_j)=w_j$
(Thm 2.6)
Need next: $T$ is inventible
Recall: Range(T)=Span{$T(v1)...T(v_n)$}=Span{$w_1,...,w_n$}
$=W$
$\Rightarrow$ $T$ is onto $\Rightarrow T$ is 1-1
$\Rightarrow T$ is inventible
$\Rightarrow V$~$W$
#### 例子
$P_3(F)$ ~ $M_{2\times2}(F)$ ~ $F^4$
dim($P_3(F)$)=dim($M_{2\times2}(F)$)=dim($F^4$)

##### 2.
$L(V,W)=\{T:T:V\xrightarrow{linear}W\}$
dim($V$)$=n$, dim($W$)$=m$

## Thm 2. 20
>dim($V$)$=n$, dim($W$)$=m$，Then $L(V,W)$~$M{m\times n}(F)$
>cor. dim($L(V,W)$)$=m\times n$
### 證明
Wanted: $\exists \Phi: L(V,W)\xrightarrow{linear\ inventible}M_{m\times n(F)}$
$\Phi(T)=[T]^\gamma_\beta$ 
Need next: $\Phi$ is linear & inventible.
1. $\Phi$ is linear (Trivial)
($\Phi(aT_1+T_2)=a\Phi(T_1)+\Phi(T_2)$)
2. We want to show $\Phi$ is onto!
For $A\in M_{m\times n}(F),\ \exists T\in L(v,w)$
such that $\Phi(T)=A$
$\beta=\{v_1,...,v_n\}$，$\gamma=\{w_1,...,w_m\}$
Let $A=(A_{ij})_{m\times n}$
Let $\exists!T:V\xrightarrow{linear}W$
$T(v_j)=\sum^m_{i=1} A_{ij}w_i$ ($1\leq j\leq n$)
$\gamma[T]^\gamma_\beta=A$
$\Phi(T)=[T]^\gamma_\beta=A$
3. $\Phi$ is 1-1
Null($\Phi$)=$\{0\}$ (0函數)
$\Phi(T)=0$ (零矩陣)
$=[T]^\gamma_\beta$
$T(v_\gamma)=0w_1+0w_2+...+0w_n$，$1\leq j\leq n$ $=0$
$\Rightarrow T(v)=0$
$\Rightarrow T=0$

## 定義
>dim($V$)$=n$，$\beta:$an ordered basis for $V$
  Define $\phi_\beta: V\rightarrow F^n$ by $\phi_beta(x)=[x]_\beta$ ，$x\in V$

## Thm 2.21
>$\phi_\beta$ is an isomorphism from $V$ to $F^n$
## 定義
>$\phi_\beta$ is called the stardard reprecentation of $V$ w.r.t.. an ordered basis $\beta$
![[Pasted image 20240904195020.png]]
> dim($V$)$=n$，dim($W$)$=m$
> $V\xrightarrow{T(linear)} W$
> $\downarrow$                  $\downarrow$
> $\phi_\beta$: $F^n$$\xrightarrow{L_A}$$F^m$ ($L_A\rightarrow A=[T]^\gamma_\beta$) 
> $L_A(x)=Ax,\ x\in F^n$
> i.e. $T:V\rightarrow W$~(看成)$L_A:F^n\rightarrow F^m$ 
> $L_A\phi_\beta=\phi_\gamma T$
> $\Rightarrow I=\phi_\gamma ^{-1}L_A\phi_\beta$

### 證明
Let $v\in V$ $L_A\phi_\beta(v)=L_A(\phi_\beta(v))=L_A([v]_\beta)=L_A([v]_\beta)$ $=A[v]^1_\beta=[T]^\gamma_\beta[v]_\beta$(矩陣、向量)=$[T(v)]_\gamma$(向量)
$=\phi_\gamma(T(v))=\phi_\gamma T(v)$

# The Change of Coordinate Matrix
二次曲線的分類
問題 $T:V\rightarrow V$ such $T$ is called a linear operator
$\beta$，$\beta'$: $V$ 的ordered basis
問: $[T]_\beta$和$[T]_{\beta'}$ 的關係為何?
$I:V\rightarrow V$($\beta$、$\beta'$) $I(v)=v$
## Thm2.22
$\Rightarrow$
1. $[I]^\beta_{\beta'}$: inventible
2. $[v]_\beta=[I]^\beta_{\beta'}[v]_{\beta'}$
### Def:
Let $Q=[I]^\beta_{\beta'}$ Then $Q$ is called a change of a coordinate matrix(That is $Q$ change $\beta'$-coordinate to $\beta$-coordinate)

### 證明
I有反函數也是自己
1. Of course!
2. Trivial!

## Thm2.24
$[T]_{\beta'}=Q^{-1}[T]_\beta Q$，$Q=[I]^\beta_{\beta'}$

### pf 
![[Pasted image 20240904203716.png]]
$T=ITI$
$\Rightarrow[T]_{\beta'}=[ITI]_{\beta'}$
$=[I]^{\beta'}_\beta[T]_\beta[I]_{\beta'}^\beta$
$=Q^{-1}[T]_\beta Q$
## 定義
> $A,B\in M_{n\times n}(F)$
> $A$ is said to be similar to $B$ 
> if $\exists Q:$ inventible. such that $B=Q^{-1}AQ$

## 應用
![[Pasted image 20240904212057.png]]
#### 轉軸公式
1.  $\begin{pmatrix}x'\\ y' \\\end{pmatrix}$$=[I]^{\beta'}_\beta$  $\begin{pmatrix}x\\ y \\\end{pmatrix}$
2.  $T(a,b)$ ? $(a,b)$

### Convince 
1. $I(v)=v$ $\Leftrightarrow [I]^{\beta'}_\beta[v]_\beta=[v]_{\beta'}$
$I:R^2\rightarrow R^2$ ($\beta$，$\beta'$={$(1,0),(0,1)$}，{$(cos\theta, sin\theta)$, $(-sin\theta, cos\theta)$}
$I((1,0))=a_1(cos\theta,sin\theta)+b_1(-sin\theta,cos\theta)$
$I((0,1))=a_2(cos\theta,sin\theta)+b_2(-sin\theta,cos\theta)$
$a_1cos\theta-b_1sin\theta=1$ ($cos\theta$)
$a_1sin\theta+b_1cos\theta=0$ ($sin\theta$)
$a_1=cos\theta$ ，$b_1=-sin\theta$
$a_2cos\theta-b_2sin\theta=1$ ($cos\theta$)
$a_2sin\theta+b_2cos\theta=0$ ($sin\theta$)
$a_2=sin\theta$ ，$b_2=-cos\theta$
$[I]^{\beta'}_\beta= \begin{pmatrix}cos\theta & sin\theta \\-sin\theta & cos\theta \\\end{pmatrix}$
$\begin{pmatrix}x'\\y'\\\end{pmatrix}=\begin{pmatrix}cos\theta & sin\theta\\-sin\theta &cos\theta\\\end{pmatrix}\begin{pmatrix}x\\y\\\end{pmatrix}$
 $x'=xcos\theta+ysin\theta$
 $y'=-xsin\theta+ycos\theta$
2. $T(a,b)=$?
![[Pasted image 20240904215050.png]]
$T=ITI$
$[T]_\beta=[I]^\beta_{\beta'}[T]_{\beta'}[I]^{\beta'}_\beta$
$T(cos\theta,sin\theta)=(cos\theta,sin\theta)$
$=1(cos\theta,sin\theta)+0(-sin\theta,cos\theta)$
$T(-sin\theta, cos\theta)=-(-sin\theta, cos\theta)$
$=0(cos\theta,sin\theta)+(-1)(-sin\theta,cos\theta)$

$[T]_{\beta'}=\begin{bmatrix}1 & 0\\0 & -1\\\end{bmatrix}$
$[I]^{\beta}_{\beta'}=\begin{pmatrix}cos\theta & -sin\theta\\sin\theta &cos\theta\\\end{pmatrix}$
$[T]_\beta=[I]^\beta_{\beta'}[T]_{\beta'}[I]^{\beta'}$
$=\begin{pmatrix}cos\theta & -sin\theta\\sin\theta&cos\theta\\\end{pmatrix} \begin{pmatrix}1 & 1\\0&-1\\\end{pmatrix} \begin{pmatrix}cos\theta & sin\theta\\-sin\theta&cos\theta\\\end{pmatrix}$
$=\begin{pmatrix}cos2\theta & sin2\theta\\sin2\theta&-cos2\theta\\\end{pmatrix}$
$[T(a,b)]=[T]_\beta \begin{pmatrix}a\\b\\\end{pmatrix}$
![[Pasted image 20240904221035.png]]


---
## 常見線性轉換(linear transformation)


# 座標化


# 矩陣表示法
## 換底公式


# Kernel 與 Image


# 矩陣的rank


# 合成與可逆

